add ptltl theorems and proofs

code-hol4/ptltl/ptltlScript.sml
@@ -1,5 +1,6 @@
 open HolKernel Parse boolLib bossLib lcsymtacs;
-open combinTheory pairTheory listTheory stringLib;
+open combinTheory pairTheory listTheory rich_listTheory stringLib;
+
 
 val _ = new_theory "ptltl";
 
@@ -46,7 +47,6 @@ End
 (* Start and End clauses are expanded versions of the original. Need an      *)
 (* extra congruence rule to extract the right termination conditions         *)
 (*---------------------------------------------------------------------------*)
-
 val _ = DefnBase.add_cong LEFT_AND_CONG;
 
 Definition bigstep_def :
@@ -92,6 +92,24 @@ Definition empty_state_def :
  empty_state = []
 End
 
+
+Definition mk_childforms_def : 
+  (mk_childforms (Eid eid) = []) /\
+  (mk_childforms (Prim b) = []) /\
+  (mk_childforms (Imp f1 f2) = [f1; f2]) /\
+  (mk_childforms (Equiv f1 f2) = [f1; f2]) /\
+  (mk_childforms (Or f1 f2) = [f1; f2]) /\
+  (mk_childforms (Xor f1 f2) = [f1; f2]) /\
+  (mk_childforms (And f1 f2) = [f1; f2]) /\
+  (mk_childforms (Since f1 f2) = [f1; f2]) /\
+  (mk_childforms (Histor f) = [f]) /\
+  (mk_childforms (Once f) = [f]) /\
+  (mk_childforms (Prev f) = [f]) /\
+  (mk_childforms (Start f) = [f]) /\
+  (mk_childforms (End f) = [f]) /\
+  (mk_childforms (Not f) = [f])
+End
+
 Definition mk_subforms_def :
   mk_subforms form = (case form
   of Eid eid => [Eid eid]
@@ -126,23 +144,20 @@ End
 
 
 Definition decide_formula_start_def :
- decide_formula_start fm st elm =
-  (case fm of
-      Eid eid     => MEM eid elm
-    | Prim b      => b
-    | Not f       => ~MEM f st
-    | Imp f1 f2   => (~MEM f1 st) \/ MEM f2 st
-    | Equiv f1 f2 => (MEM f1 st = MEM f2 st)
-    | Or f1 f2    => (MEM f1 st \/ MEM f2 st)
-    | Xor f1 f2   => ~(MEM f1 st = MEM f2 st)
-    | And f1 f2   => (MEM f1 st /\ MEM f2 st)
-    | Since f1 f2 => (MEM f1 st /\ MEM f2 st)
-    | Histor f    => MEM f st
-    | Once f      => MEM f st
-    | Prev f      => MEM f st
-    | Start f     => F
-    | End f       => F
-  )
+  (decide_formula_start (Eid eid) st elm     <=> MEM eid elm) /\
+  (decide_formula_start (Prim b) st elm      <=> b) /\
+  (decide_formula_start (Not f) st elm       <=> ~MEM f st) /\
+  (decide_formula_start (Imp f1 f2) st elm   <=> (~ MEM f1 st) \/ MEM f2 st) /\
+  (decide_formula_start (Equiv f1 f2) st elm <=> (MEM f1 st = MEM f2 st)) /\
+  (decide_formula_start (Or f1 f2) st elm    <=> (MEM f1 st \/ MEM f2 st)) /\
+  (decide_formula_start (Xor f1 f2) st elm   <=> ~(MEM f1 st = MEM f2 st)) /\
+  (decide_formula_start (And f1 f2) st elm   <=> (MEM f1 st /\ MEM f2 st)) /\
+  (decide_formula_start (Since f1 f2) st elm <=> (MEM f1 st /\ MEM f2 st)) /\
+  (decide_formula_start (Histor f) st elm    <=> MEM f st) /\
+  (decide_formula_start (Once f) st elm      <=> MEM f st) /\
+  (decide_formula_start (Prev f) st elm      <=> MEM f st) /\
+  (decide_formula_start (Start f) st elm     <=> F) /\
+  (decide_formula_start (End f) st elm       <=> F)
 End
 
 Definition decide_formula_def :
@@ -169,7 +184,7 @@ End
 Definition transition_start_def :
  transition_start sforms elm =
    FOLDL
-     (\st_acc fm.
+     (\ st_acc fm .
          let decision = decide_formula_start fm st_acc elm
          in (if decision then
            fm :: st_acc
@@ -184,7 +199,7 @@ End
 Definition transition_def:
  transition sforms st elm =
    FOLDL
-     (\st_acc fm.
+     (\ st_acc fm .
          let decision = decide_formula fm st st_acc elm
          in (if decision then
            fm :: st_acc
@@ -196,11 +211,11 @@ Definition transition_def:
      sforms
 End
 
-Definition dfa_loop_def :
- dfa_loop delta form elms st =
-   (case elms
+Definition smallstep_loop_def :
+ smallstep_loop delta form trace st =
+   (case trace 
      of [] => MEM form st
-      | elm :: elms' => dfa_loop delta form elms' (delta st elm))
+      | elm :: trace' => smallstep_loop delta form trace' (delta st elm))
 End
 
 
@@ -212,7 +227,7 @@ Definition smallstep_def :
       delta = transition subforms;
    in \ elms. case elms
               of [] => MEM form (delta_start other_elm)
-               | elm :: elms' => dfa_loop delta form elms' (delta_start elm)
+               | elm :: elms' => smallstep_loop delta form elms' (delta_start elm)
 End
 
 Definition  mk_power_list_def :
@@ -350,10 +365,6 @@ Definition mk_table_data_def :
 
 End
 
-Definition table_transition_def:
-  table_transition table state_idx elm_idx = EL elm_idx (EL state_idx table)
-End
-
 
 (* This should stay at the SML level
 Definition to_dotgraph_def :
@@ -414,5 +425,1645 @@ Definition to_dotgraph_def :
   )
 End
 *)
+
+Definition table_transition_def:
+  table_transition table state_idx elm_idx = EL elm_idx (EL state_idx table)
+End
+
+
+Definition dfa_loop_def :
+  dfa_loop table state_idx idx_trace = (case idx_trace of [] => state_idx |
+    (elm_idx :: idx_trace') => (
+      dfa_loop table (table_transition table state_idx elm_idx) idx_trace'
+    )
+  )
+End
+
+
+Definition dfa_def :
+ dfa form =
+   (let
+      relational_data = mk_relational_data form T;
+      (state_to_index, elm_to_idx, finals, table, start_idx) = mk_table_data relational_data;
+      is_accepted = (\ idx . EL idx finals);
+   in
+     (\ trace . (let
+       idx_trace = MAP (\ elm . elm_to_idx elm) trace;
+     in case idx_trace of
+       [] => is_accepted (table_transition table start_idx (elm_to_idx other_elm)) |
+       elm_idx :: idx_trace' =>
+         is_accepted (dfa_loop table start_idx (elm_idx :: idx_trace'))
+     ))
+   )
+End
+
+
+Definition transition_start_right_def :
+ transition_start_right sforms elm =
+   FOLDR
+     (\ fm st_acc .
+         let decision = decide_formula_start fm st_acc elm
+         in (if decision then
+           fm :: st_acc
+         else
+           st_acc
+         )
+     )
+     empty_state
+     sforms
+End
+
+
+Definition transition_start_rec_def :
+ (transition_start_rec [] elm = empty_state) /\
+ (transition_start_rec (fm :: forms) elm =
+   (if (decide_formula_start fm (transition_start_rec forms elm) elm) then
+     fm :: (transition_start_rec forms elm)
+   else
+     (transition_start_rec forms elm)
+   )
+ )
+End
+
+
+Definition list_step_start_def :
+  (list_step_start [] elm form = F) /\
+  (list_step_start (f :: fs) elm form =
+  (if (form <> f) then
+    (list_step_start fs elm form)
+  else
+    (∀ eid . f = Eid eid ==> MEM eid elm) /\
+    (∀ b . f = Prim b ==> b) /\
+
+    (∀ form1 form2 . f = Imp form1 form2 ==>
+      ~ list_step_start fs elm form1 \/ list_step_start fs elm form2 
+    ) /\
+
+    (∀ form1 form2 . f = Equiv form1 form2 ==>
+      list_step_start fs elm form1 = list_step_start fs elm form2 
+    ) /\
+
+    (∀ form1 form2 . f = Or form1 form2 ==>
+      list_step_start fs elm form1 \/ list_step_start fs elm form2 
+    ) /\
+
+    (∀ form1 form2 . f = Xor form1 form2 ==>
+      list_step_start fs elm form1 <> list_step_start fs elm form2 
+    ) /\
+
+    (∀ form1 form2 . f = And form1 form2 ==>
+      list_step_start fs elm form1 /\ list_step_start fs elm form2 
+    ) /\
+
+    (∀ form1 form2 . f = Since form1 form2 ==>
+      list_step_start fs elm form1 /\ list_step_start fs elm form2 
+    ) /\
+
+    (∀ form' . f = Histor form' ==>
+      list_step_start fs elm form' 
+    ) /\
+
+    (∀ form' . f = Once form' ==>
+      list_step_start fs elm form' 
+    ) /\
+
+    (∀ form' . f = Prev form' ==>
+      list_step_start fs elm form' 
+    ) /\
+
+    (∀ form' . f = Start form' ==> F) /\
+
+    (∀ form' . f = End form' ==> F) /\
+
+    (∀ form' . f = Not form' ==> ~ list_step_start fs elm form')
+
+  ))
+
+End
+
+(*
+    (EXISTS (\ f' . MEM f' (mk_childforms f)) fs) /\
+*)
+
+Definition list_wellformed_def :
+  (list_wellformed [] <=> T) /\
+  (list_wellformed (f::fs) <=>
+    (EVERY (\ f' . MEM f' fs) (mk_childforms f)) /\
+    (EVERY (\ f' . ~MEM f (mk_childforms f')) fs) /\
+    (~ MEM f fs) /\
+    (list_wellformed fs)
+  )
+End
+
+
+
+val transition_start_REVERSE_right_equiv_thm = Q.store_thm (
+  "transition_start_REVERSE_right_equiv_thm",
+  (`∀ sforms elm . 
+    transition_start (REVERSE sforms) elm = transition_start_right sforms elm
+  `),
+  rw [transition_start_def, transition_start_right_def, FOLDL_REVERSE]
+)
+
+
+val transition_start_rec_thm = Q.store_thm (
+  "transition_start_rec_thm",
+  `∀ sforms elm . transition_start_rec sforms elm = transition_start_right sforms elm`,
+  Induct_on `sforms` >> fs [transition_start_rec_def, transition_start_right_def]
+)
+
+val transition_start_REVERSE_rec_equiv_thm = Q.store_thm (
+  "transition_start_REVERSE_rec_equiv_thm",
+  (`∀ sforms elm . 
+    transition_start (REVERSE sforms) elm = transition_start_rec sforms elm
+  `),
+  metis_tac [transition_start_REVERSE_right_equiv_thm, transition_start_rec_thm]
+)
+
+
+val MEM_subforms_refl_thm = Q.store_thm (
+  "MEM_subforms_refl_thm",
+  `∀ f . MEM f (mk_subforms f)`,
+  (GEN_TAC >> ONCE_REWRITE_TAC [mk_subforms_def] >> CASE_TAC >> fs [])
+)
+
+
+val MEM_subforms_onestep_thm = Q.store_thm (
+  "MEM_subforms_onestep_thm",
+  (`∀ x y .
+    MEM x (mk_childforms y)
+    ==> 
+    MEM x (mk_subforms y)
+  `),
+  Cases_on `y` >>
+  rw [mk_childforms_def, Once mk_subforms_def] >>
+  rw [MEM_subforms_refl_thm]
+)
+
+
+val MEM_subforms_multistep_thm = Q.store_thm (
+  "MEM_subforms_multistep_thm",
+  (`∀ x y z .
+    MEM x (mk_childforms y) /\ MEM y (mk_subforms z) ==> 
+    MEM x (mk_subforms z)
+  `),
+  Cases_on `y` >> rw [mk_childforms_def] >> ( 
+     Induct_on `z` >> (
+       TRY (ONCE_REWRITE_TAC [mk_subforms_def] >> CASE_TAC >> rw [] >> rw []) >>
+       TRY (metis_tac [MEM_subforms_refl_thm]) >>
+       rw [mk_subforms_def]
+     )
+  )
+)
+
+
+val MEM_subforms_elim_thm = Q.store_thm (
+  "MEM_subforms_elim_thm",
+  (`∀ x z .
+    MEM x (mk_subforms z) ==> 
+    (
+      (x = z) \/
+      (MEM x (mk_childforms z)) \/ 
+      (∃y. MEM x (mk_childforms y) /\ MEM y (mk_subforms z))
+    )
+  `),
+  rw [] >>
+  Induct_on `z` >| [
+    fs [Once mk_subforms_def, mk_childforms_def],
+    fs [Once mk_subforms_def, mk_childforms_def]
+  ] @ (List.tabulate (12, fn _ =>
+
+    DISCH_TAC >>
+    POP_ASSUM (fn thm =>
+      MP_TAC (REWRITE_RULE [Once mk_subforms_def] thm)
+    ) >> fs [] >> DISCH_TAC >>
+
+
+    REWRITE_TAC [Once mk_childforms_def] >>
+    REWRITE_TAC [Once mk_subforms_def] >>
+    rw [] >> fs [] >>
+    metis_tac [MEM_subforms_refl_thm]
+  ))
+)
+
+
+val MEM_subforms_thm = Q.store_thm (
+  "MEM_subforms_thm",
+  (`∀ x z .
+    MEM x (mk_subforms z) <=> (
+      x = z \/
+      (MEM x (mk_childforms z)) \/ 
+      (∃ y . (MEM x (mk_childforms y) /\ MEM y (mk_subforms z)))
+    )
+  `),
+  metis_tac [
+    MEM_subforms_elim_thm,
+    MEM_subforms_refl_thm,
+    MEM_subforms_onestep_thm,
+    MEM_subforms_multistep_thm
+  ]
+)
+
+
+val MEM_childforms_anti_refl_thm = Q.store_thm (
+  "MEM_childforms_anti_refl_thm",
+  (` ∀ x y .
+    MEM x (mk_childforms y) ==>
+    ~ (x = y)
+  `),
+  (
+  Cases_on `y` >> rw [mk_childforms_def] >>
+  TRY (Q.SPEC_TAC (`f0`, `f0`) >> Induct_on `f` >> fs [] >> metis_tac []) >>
+  TRY (Q.SPEC_TAC (`f`, `f`) >> Induct_on `f0` >> fs [] >> metis_tac [])
+  )
+)
+
+
+val MEM_subforms_acyclic_thm = Q.store_thm (
+  "MEM_subforms_acyclic_thm",
+  (`∀ x y .
+    (MEM x (mk_childforms y)) ==>
+    ~ (MEM y (mk_subforms x))
+  `),
+  (let
+  
+    fun form_tac_pair_1 con a1 a2 =
+    (
+      DISCH_TAC >>
+      ASSUME_TAC (Q.SPECL [`(^(con) ^(a1) ^(a2))`, `y`, `^(a1)`] MEM_subforms_multistep_thm) >>
+      POP_ASSUM (fn imp_thm => POP_ASSUM (fn arg1_thm => POP_ASSUM (fn arg2_thm =>
+        MP_TAC (MP imp_thm (CONJ arg2_thm arg1_thm)) 
+      ))) >>
+      POP_ASSUM (fn _ => POP_ASSUM (fn thm => 
+        MP_TAC (Q.SPEC `(^(con) ^(a1) ^(a2))` thm) 
+      )) >>
+      rw [mk_childforms_def]
+    )
+    
+    fun form_tac_pair_2 con a1 a2 =
+    (
+      DISCH_TAC >>
+      ASSUME_TAC (Q.SPECL [`(^(con) ^(a1) ^(a2))`, `y`, `^(a2)`] MEM_subforms_multistep_thm) >>
+      POP_ASSUM (fn imp_thm => POP_ASSUM (fn arg1_thm => POP_ASSUM (fn arg2_thm =>
+        MP_TAC (MP imp_thm (CONJ arg2_thm arg1_thm)) 
+      ))) >>
+      POP_ASSUM (fn thm => POP_ASSUM (fn _ => 
+        MP_TAC (Q.SPEC `(^(con) ^(a1) ^(a2))` thm) 
+      )) >>
+      rw [mk_childforms_def]
+    )
+    
+    fun form_tac con a =
+    (
+      DISCH_TAC >>
+      ASSUME_TAC (Q.SPECL [`(^(con) ^(a))`, `y`, `^(a)`] MEM_subforms_multistep_thm) >>
+      POP_ASSUM (fn imp_thm => POP_ASSUM (fn arg1_thm => POP_ASSUM (fn arg2_thm =>
+        MP_TAC (MP imp_thm (CONJ arg2_thm arg1_thm)) 
+      ))) >>
+      POP_ASSUM (fn thm => 
+        MP_TAC (Q.SPEC `(^(con) ^(a))` thm) 
+      ) >>
+      rw [mk_childforms_def]
+    )
+  
+  in
+    Induct_on `x` >|
+    (
+       [fs [mk_subforms_def, mk_childforms_def], fs [mk_subforms_def, mk_childforms_def]] @
+
+       (List.map (fn con =>
+         ONCE_REWRITE_TAC [mk_subforms_def] >> CASE_TAC >> rw [] >|
+         [
+           fs [MEM_childforms_anti_refl_thm],
+           (form_tac_pair_1 con ``f : formula`` ``f0 : formula``),
+           (form_tac_pair_2 con ``f : formula`` ``f0 : formula``)
+         ]
+       ) [``Imp``, ``Equiv``, ``Or``, ``Xor``, ``And``, ``Since``]) @
+
+       (List.map (fn con =>
+         ONCE_REWRITE_TAC [mk_subforms_def] >> CASE_TAC >> rw [] >|
+         [
+           fs [MEM_childforms_anti_refl_thm],
+           (form_tac con ``f : formula``)
+         ]
+       ) [``Histor``,``Once``, ``Prev``, ``Start``, ``End``, ``Not``])
+    )
+
+  end)
+)
+
+
+val subforms_self_first_thm = Q.store_thm (
+  "subforms_self_first_thm",
+  `∀ f . ∃ fs . mk_subforms f = f :: fs`,
+  Cases_on `f` >> rw [Once (mk_subforms_def)]
+)
+
+val MEM_subforms_self_thm = Q.store_thm (
+  "MEM_subforms_self_thm",
+  `∀ f . MEM f (mk_subforms f)`,
+  Cases_on `f` >> rw [Once (mk_subforms_def)]
+)
+
+val nub_subforms_self_first_thm = Q.store_thm (
+  "nub_subforms_self_first_thm",
+  `∀ f . ∃ fs . nub (mk_subforms f) = f :: fs`,
+  Cases_on `f` >> rw [
+    Once (mk_subforms_def), nub_def,
+    MEM_subforms_acyclic_thm, mk_childforms_def
+  ]
+)
+
+val nub_subforms_MEM_thm = Q.store_thm (
+  "nub_subforms_MEM_thm",
+  `∀ f . ∃ fs . nub (mk_subforms f) = fs /\ MEM f fs`,
+  Cases_on `f` >> rw [
+    Once (mk_subforms_def), nub_def,
+    MEM_subforms_acyclic_thm, mk_childforms_def
+  ]
+)
+
+
+val MEM_nub_thm = Q.store_thm (
+  "MEM_nub_thm",
+  (`∀ x xs . MEM x (nub xs) <=> MEM x xs `),
+  Induct_on `xs` >> rw [nub_def]
+)
+
+val FILTER_nub_thm = Q.store_thm (
+  "FILTER_nub_thm",
+  `∀ l P . FILTER P (nub l) = nub (FILTER P l)`,
+  Induct_on `l` >> rw [nub_def, FILTER, MEM_FILTER]
+)
+
+
+val MEM_transition_start_rec_constrained_thm = Q.store_thm (
+  "MEM_transition_start_rec_constrained_thm",
+  `∀ f fs elm .
+    ~MEM f fs ==>
+    ~ MEM f (transition_start_rec fs elm)
+  `,
+  rw [] >>
+  Induct_on `fs` >> rw [transition_start_rec_def, empty_state_def] 
+)
+
+
+val MEM_transition_start_rec_APPEND_thm = Q.store_thm (
+  "MEM_transition_start_rec_APPEND_thm",
+  (`∀ f fs xs .
+     MEM f (transition_start_rec fs other_elm) ==>
+     MEM f (transition_start_rec (xs ++ fs) other_elm)
+  `),
+  Induct_on `xs` >> rw [transition_start_rec_def]
+)
+
+
+
+
+
+val MEM_transition_start_rec_imp_Q_thm = Q.store_thm (
+  "MEM_transition_start_rec_imp_Q_thm",
+  (`∀ form fs form' fs' .
+    MEM form' (transition_start_rec fs' other_elm) ==>
+    list_wellformed fs ==>
+    list_wellformed fs' ==>
+    (MEM (Imp form form') (transition_start_rec
+      (Imp form form':: (FILTER (λx. ~MEM x (fs')) fs ++ fs'))
+      other_elm
+    ))
+  `),
+  GEN_TAC >> GEN_TAC >> GEN_TAC >> GEN_TAC >>
+  DISCH_TAC >> DISCH_TAC >> DISCH_TAC >>
+  REWRITE_TAC [Once transition_start_rec_def] >>
+  (`∀ st_acc . decide_formula_start (Imp form form') st_acc other_elm <=>
+    (~ MEM form st_acc \/ MEM form' st_acc)
+  `) by (rw [decide_formula_start_def]) >>
+  POP_ASSUM (fn rw_thm => REWRITE_TAC [rw_thm]) >>
+  fs [MEM_transition_start_rec_APPEND_thm]
+)
+
+
+
+
+
+
+val MEM_transition_start_rec_drop_thm = Q.store_thm (
+  "MEM_transition_start_rec_drop_thm",
+  (`∀ f fs xs .
+     list_wellformed (xs ++ (f :: fs)) ==>
+     MEM f (transition_start_rec (xs ++ (f :: fs)) other_elm) ==>
+     MEM f (transition_start_rec (f :: fs) other_elm)
+  `),
+  rw [] >>
+  Induct_on `xs` >| [
+    rw [] 
+    ,
+
+    GEN_TAC >>
+    fs [Once CONS_APPEND] >>
+    DISCH_TAC >>
+    POP_ASSUM (fn thm =>
+      ASSUME_TAC (REWRITE_RULE [list_wellformed_def] thm)
+    ) >>
+
+    DISCH_TAC >>
+    POP_ASSUM (fn thm =>
+      ASSUME_TAC (REWRITE_RULE [transition_start_rec_def] thm)
+    ) >>
+
+    Cases_on `decide_formula_start h (transition_start_rec (xs ++ f::fs) other_elm) other_elm` >>
+    (fs [EVERY_MEM, EXISTS_MEM] >> fs [])
+
+  ] 
+)
+
+
+val list_wellformed_anti_super_thm = Q.store_thm (
+  "list_wellformed_anti_super_thm",
+  (`∀ x xs f .
+    list_wellformed (x :: xs) ==>
+    MEM x (mk_childforms f) ==>
+    ~ MEM f (x :: xs)
+  `),
+  GEN_TAC >> GEN_TAC >> GEN_TAC >>
+  DISCH_TAC >> DISCH_TAC >>
+  (rw [] >- rw [MEM_childforms_anti_refl_thm]) >>
+  fs [list_wellformed_def, EVERY_MEM] >>
+  (Cases_on `xs` >- fs []) >>
+  fs [] >> (
+    qpat_x_assum `∀f'. f' = h ∨ MEM f' t ⇒ ¬MEM x (mk_childforms f')` (fn thm =>
+      ASSUME_TAC (Q.SPEC `f` thm)
+    ) >>
+    metis_tac []
+  )
+)
+
+val list_step_start_Eid_elim_thm = Q.store_thm (
+  "list_step_start_Eid_elim_thm",
+  (`∀ s forms .
+    ~ list_step_start forms other_elm (Eid s)
+  `),
+  rw [] >>
+  Induct_on `forms`
+  >| [
+    fs [list_step_start_def, other_elm_def, empty_state_def]
+    ,
+
+    GEN_TAC >>
+    fs [list_step_start_def, other_elm_def, empty_state_def] >>
+    rw [] >>
+    (Cases_on `h = Eid s` >> fs [])
+  ]
+)
+
+val list_step_start_Prim_false_elim_thm = Q.store_thm (
+  "list_step_start_Prim_false_elim_thm",
+  (`∀ forms .
+    ~ list_step_start forms other_elm (Prim F)
+  `),
+  rw [] >>
+  Induct_on `forms`
+  >| [
+    fs [list_step_start_def, other_elm_def, empty_state_def]
+    ,
+
+    GEN_TAC >>
+    fs [list_step_start_def, other_elm_def, empty_state_def] >>
+    rw [] >>
+    (Cases_on `h = Prim F` >> fs [])
+  ]
+)
+
+val list_step_start_constrained_thm = Q.store_thm (
+  "list_step_start_constrained_thm",
+  `∀ forms elm form .
+    list_step_start forms elm form ==> 
+    MEM form forms
+  `,
+  rw [] >>
+  Induct_on `forms` >> rw [list_step_start_def, empty_state_def] 
+)
+
+
+val list_step_start_Imp_elim_thm = Q.store_thm (
+  "list_step_start_Imp_elim_thm",
+  (`∀ forms f1 f2 .
+    list_wellformed forms ==>
+    list_step_start forms other_elm (Imp f1 f2) ==>
+    list_step_start forms other_elm f1 ==>
+    list_step_start forms other_elm f2 
+  `),
+  rw [] >>
+  Induct_on `forms`
+  >| [
+    rw [list_step_start_def]
+    ,
+
+    GEN_TAC >>
+    Cases_on `h = Imp f1 f2`
+    >| [
+      `h <> f1` by (fs [MEM_childforms_anti_refl_thm, mk_childforms_def]) >>
+      `h <> f2` by (fs [MEM_childforms_anti_refl_thm, mk_childforms_def]) >>
+      rw [list_step_start_def] >>
+      fs []
+      ,
+
+      DISCH_TAC >> POP_ASSUM (fn thm =>
+        ASSUME_TAC (REWRITE_RULE [list_wellformed_def] thm)
+      ) >>
+      fs [] >>
+
+      rw [Once list_step_start_def] >>
+      fs [] >>
+
+      `MEM (Imp f1 f2) forms` by (metis_tac [list_step_start_constrained_thm]) >>
+      fs [EVERY_MEM] >>
+
+      qpat_assum `MEM (Imp f1 f2) forms` (fn arg_thm =>
+      qpat_assum `∀f'. MEM f' forms ==> ~MEM h (mk_childforms f')` (fn thm =>
+        ASSUME_TAC (MP (Q.SPEC `Imp f1 f2` thm) arg_thm)
+      )) >>
+      fs [mk_childforms_def] >>
+      fs [list_step_start_def] >>
+      rw [list_step_start_def] 
+    ]
+
+  ]
+)
+
+val list_step_start_Equiv_elim_thm = Q.store_thm (
+  "list_step_start_Equiv_elim_thm",
+  (`∀ forms f1 f2 .
+    list_wellformed forms ==>
+    list_step_start forms other_elm (Equiv f1 f2) ==>
+    list_step_start forms other_elm f1 = list_step_start forms other_elm f2 
+  `),
+  rw [] >>
+  Induct_on `forms`
+  >| [
+    rw [list_step_start_def]
+    ,
+
+    GEN_TAC >>
+    Cases_on `h = Equiv f1 f2`
+    >| [
+      `h <> f1` by (fs [MEM_childforms_anti_refl_thm, mk_childforms_def]) >>
+      `h <> f2` by (fs [MEM_childforms_anti_refl_thm, mk_childforms_def]) >>
+      rw [list_step_start_def] >>
+      fs []
+      ,
+
+      DISCH_TAC >> POP_ASSUM (fn thm =>
+        ASSUME_TAC (REWRITE_RULE [list_wellformed_def] thm)
+      ) >>
+      fs [] >>
+
+      rw [Once list_step_start_def] >>
+      fs [] >>
+
+      `MEM (Equiv f1 f2) forms` by (metis_tac [list_step_start_constrained_thm]) >>
+      fs [EVERY_MEM] >>
+
+      qpat_assum `MEM (Equiv f1 f2) forms` (fn arg_thm =>
+      qpat_assum `∀f'. MEM f' forms ==> ~MEM h (mk_childforms f')` (fn thm =>
+        ASSUME_TAC (MP (Q.SPEC `Equiv f1 f2` thm) arg_thm)
+      )) >>
+      fs [mk_childforms_def] >>
+      fs [list_step_start_def] >>
+      rw [list_step_start_def] 
+    ]
+
+  ]
+)
+
+val list_step_start_Or_elim_thm = Q.store_thm (
+  "list_step_start_Or_elim_thm",
+  (`∀ forms f1 f2 .
+    list_wellformed forms ==>
+    list_step_start forms other_elm (Or f1 f2) ==>
+    list_step_start forms other_elm f1 \/ list_step_start forms other_elm f2 
+  `),
+  rw [] >>
+  Induct_on `forms`
+  >| [
+    rw [list_step_start_def]
+    ,
+
+    GEN_TAC >>
+    Cases_on `h = Or f1 f2`
+    >| [
+      `h <> f1` by (fs [MEM_childforms_anti_refl_thm, mk_childforms_def]) >>
+      `h <> f2` by (fs [MEM_childforms_anti_refl_thm, mk_childforms_def]) >>
+      rw [list_step_start_def] >>
+      fs []
+      ,
+
+      DISCH_TAC >> POP_ASSUM (fn thm =>
+        ASSUME_TAC (REWRITE_RULE [list_wellformed_def] thm)
+      ) >>
+      fs [] >>
+
+      rw [Once list_step_start_def] >>
+      fs [] >>
+
+      `MEM (Or f1 f2) forms` by (metis_tac [list_step_start_constrained_thm]) >>
+      fs [EVERY_MEM] >>
+
+      qpat_assum `MEM (Or f1 f2) forms` (fn arg_thm =>
+      qpat_assum `∀f'. MEM f' forms ==> ~MEM h (mk_childforms f')` (fn thm =>
+        ASSUME_TAC (MP (Q.SPEC `Or f1 f2` thm) arg_thm)
+      )) >>
+      fs [mk_childforms_def] >>
+      fs [list_step_start_def] >>
+      rw [list_step_start_def] 
+    ]
+
+  ]
+)
+
+val list_step_start_Xor_elim_thm = Q.store_thm (
+  "list_step_start_Xor_elim_thm",
+  (`∀ forms f1 f2 .
+    list_wellformed forms ==>
+    list_step_start forms other_elm (Xor f1 f2) ==>
+    list_step_start forms other_elm f1 <> list_step_start forms other_elm f2 
+  `),
+  rw [] >>
+  Induct_on `forms`
+  >| [
+    rw [list_step_start_def]
+    ,
+
+    GEN_TAC >>
+    Cases_on `h = Xor f1 f2`
+    >| [
+      `h <> f1` by (fs [MEM_childforms_anti_refl_thm, mk_childforms_def]) >>
+      `h <> f2` by (fs [MEM_childforms_anti_refl_thm, mk_childforms_def]) >>
+      rw [list_step_start_def] >>
+      fs []
+      ,
+
+      DISCH_TAC >> POP_ASSUM (fn thm =>
+        ASSUME_TAC (REWRITE_RULE [list_wellformed_def] thm)
+      ) >>
+      fs [] >>
+
+      rw [Once list_step_start_def] >>
+      fs [] >>
+
+      `MEM (Xor f1 f2) forms` by (metis_tac [list_step_start_constrained_thm]) >>
+      fs [EVERY_MEM] >>
+
+      qpat_assum `MEM (Xor f1 f2) forms` (fn arg_thm =>
+      qpat_assum `∀f'. MEM f' forms ==> ~MEM h (mk_childforms f')` (fn thm =>
+        ASSUME_TAC (MP (Q.SPEC `Xor f1 f2` thm) arg_thm)
+      )) >>
+      fs [mk_childforms_def] >>
+      fs [list_step_start_def] >>
+      rw [list_step_start_def] 
+    ]
+
+  ]
+)
+
+val list_step_start_And_elim_thm = Q.store_thm (
+  "list_step_start_And_elim_thm",
+  (`∀ forms f1 f2 .
+    list_wellformed forms ==>
+    list_step_start forms other_elm (And f1 f2) ==>
+    list_step_start forms other_elm f1 /\ list_step_start forms other_elm f2 
+  `),
+  GEN_TAC >> GEN_TAC >> GEN_TAC >>
+  Induct_on `forms`
+  >| [
+    rw [list_step_start_def]
+    ,
+
+    GEN_TAC >>
+    Cases_on `h = And f1 f2`
+    >| [
+      `h <> f1` by (fs [MEM_childforms_anti_refl_thm, mk_childforms_def]) >>
+      `h <> f2` by (fs [MEM_childforms_anti_refl_thm, mk_childforms_def]) >>
+      rw [list_step_start_def] >>
+      fs []
+      ,
+
+      DISCH_TAC >> POP_ASSUM (fn thm =>
+        ASSUME_TAC (REWRITE_RULE [list_wellformed_def] thm)
+      ) >>
+      fs [] >>
+
+      rw [Once list_step_start_def] >>
+      fs [] >>
+
+      `MEM (And f1 f2) forms` by (metis_tac [list_step_start_constrained_thm]) >>
+      fs [EVERY_MEM] >>
+
+      qpat_assum `MEM (And f1 f2) forms` (fn arg_thm =>
+      qpat_assum `∀f'. MEM f' forms ==> ~MEM h (mk_childforms f')` (fn thm =>
+        ASSUME_TAC (MP (Q.SPEC `And f1 f2` thm) arg_thm)
+      )) >>
+      fs [mk_childforms_def] >>
+      fs [list_step_start_def] >>
+      rw [list_step_start_def] 
+    ]
+
+  ]
+)
+
+val list_step_start_Since_elim_thm = Q.store_thm (
+  "list_step_start_Since_elim_thm",
+  (`∀ forms f1 f2 .
+    list_wellformed forms ==>
+    list_step_start forms other_elm (Since f1 f2) ==>
+    list_step_start forms other_elm f1 /\ list_step_start forms other_elm f2 
+  `),
+  GEN_TAC >> GEN_TAC >> GEN_TAC >>
+  Induct_on `forms`
+  >| [
+    rw [list_step_start_def]
+    ,
+
+    GEN_TAC >>
+    Cases_on `h = Since f1 f2`
+    >| [
+      `h <> f1` by (fs [MEM_childforms_anti_refl_thm, mk_childforms_def]) >>
+      `h <> f2` by (fs [MEM_childforms_anti_refl_thm, mk_childforms_def]) >>
+      rw [list_step_start_def] >>
+      fs []
+      ,
+
+      DISCH_TAC >> POP_ASSUM (fn thm =>
+        ASSUME_TAC (REWRITE_RULE [list_wellformed_def] thm)
+      ) >>
+      fs [] >>
+
+      rw [Once list_step_start_def] >>
+      fs [] >>
+
+      `MEM (Since f1 f2) forms` by (metis_tac [list_step_start_constrained_thm]) >>
+      fs [EVERY_MEM] >>
+
+      qpat_assum `MEM (Since f1 f2) forms` (fn arg_thm =>
+      qpat_assum `∀f'. MEM f' forms ==> ~MEM h (mk_childforms f')` (fn thm =>
+        ASSUME_TAC (MP (Q.SPEC `Since f1 f2` thm) arg_thm)
+      )) >>
+      fs [mk_childforms_def] >>
+      fs [list_step_start_def] >>
+      rw [list_step_start_def] 
+    ]
+
+  ]
+)
+
+
+val list_step_start_Histor_elim_thm = Q.store_thm (
+  "list_step_start_Histor_elim_thm",
+  (`∀ forms f .
+    list_wellformed forms ==>
+    list_step_start forms other_elm (Histor f) ==>
+    list_step_start forms other_elm f 
+  `),
+  rw [] >>
+  Induct_on `forms`
+  >| [
+    rw [list_step_start_def]
+    ,
+
+    GEN_TAC >>
+    Cases_on `h = Histor f`
+    >| [
+      `h <> f` by (fs [MEM_childforms_anti_refl_thm, mk_childforms_def]) >>
+      rw [list_step_start_def] >>
+      fs []
+      ,
+
+      DISCH_TAC >> POP_ASSUM (fn thm =>
+        ASSUME_TAC (REWRITE_RULE [list_wellformed_def] thm)
+      ) >>
+      fs [] >>
+
+      rw [Once list_step_start_def] >>
+      fs [] >>
+
+      `MEM (Histor f) forms` by (metis_tac [list_step_start_constrained_thm]) >>
+      fs [EVERY_MEM] >>
+
+      qpat_assum `MEM (Histor f) forms` (fn arg_thm =>
+      qpat_assum `∀f'. MEM f' forms ==> ~MEM h (mk_childforms f')` (fn thm =>
+        ASSUME_TAC (MP (Q.SPEC `Histor f` thm) arg_thm)
+      )) >>
+      fs [mk_childforms_def] >>
+      fs [list_step_start_def] >>
+      rw [list_step_start_def] 
+    ]
+
+  ]
+)
+
+val list_step_start_Once_elim_thm = Q.store_thm (
+  "list_step_start_Once_elim_thm",
+  (`∀ forms f .
+    list_wellformed forms ==>
+    list_step_start forms other_elm (Once f) ==>
+    list_step_start forms other_elm f 
+  `),
+  rw [] >>
+  Induct_on `forms`
+  >| [
+    rw [list_step_start_def]
+    ,
+
+    GEN_TAC >>
+    Cases_on `h = Once f`
+    >| [
+      `h <> f` by (fs [MEM_childforms_anti_refl_thm, mk_childforms_def]) >>
+      rw [list_step_start_def] >>
+      fs []
+      ,
+
+      DISCH_TAC >> POP_ASSUM (fn thm =>
+        ASSUME_TAC (REWRITE_RULE [list_wellformed_def] thm)
+      ) >>
+      fs [] >>
+
+      rw [Once list_step_start_def] >>
+      fs [] >>
+
+      `MEM (Once f) forms` by (metis_tac [list_step_start_constrained_thm]) >>
+      fs [EVERY_MEM] >>
+
+      qpat_assum `MEM (Once f) forms` (fn arg_thm =>
+      qpat_assum `∀f'. MEM f' forms ==> ~MEM h (mk_childforms f')` (fn thm =>
+        ASSUME_TAC (MP (Q.SPEC `Once f` thm) arg_thm)
+      )) >>
+      fs [mk_childforms_def] >>
+      fs [list_step_start_def] >>
+      rw [list_step_start_def] 
+    ]
+
+  ]
+)
+
+val list_step_start_Prev_elim_thm = Q.store_thm (
+  "list_step_start_Prev_elim_thm",
+  (`∀ forms f .
+    list_wellformed forms ==>
+    list_step_start forms other_elm (Prev f) ==>
+    list_step_start forms other_elm f 
+  `),
+  rw [] >>
+  Induct_on `forms`
+  >| [
+    rw [list_step_start_def]
+    ,
+
+    GEN_TAC >>
+    Cases_on `h = Prev f`
+    >| [
+      `h <> f` by (fs [MEM_childforms_anti_refl_thm, mk_childforms_def]) >>
+      rw [list_step_start_def] >>
+      fs []
+      ,
+
+      DISCH_TAC >> POP_ASSUM (fn thm =>
+        ASSUME_TAC (REWRITE_RULE [list_wellformed_def] thm)
+      ) >>
+      fs [] >>
+
+      rw [Once list_step_start_def] >>
+      fs [] >>
+
+      `MEM (Prev f) forms` by (metis_tac [list_step_start_constrained_thm]) >>
+      fs [EVERY_MEM] >>
+
+      qpat_assum `MEM (Prev f) forms` (fn arg_thm =>
+      qpat_assum `∀f'. MEM f' forms ==> ~MEM h (mk_childforms f')` (fn thm =>
+        ASSUME_TAC (MP (Q.SPEC `Prev f` thm) arg_thm)
+      )) >>
+      fs [mk_childforms_def] >>
+      fs [list_step_start_def] >>
+      rw [list_step_start_def] 
+    ]
+
+  ]
+)
+
+val list_step_start_Not_elim_thm = Q.store_thm (
+  "list_step_start_Not_elim_thm",
+  (`∀ forms f .
+    list_wellformed forms ==>
+    list_step_start forms other_elm (Not f) ==>
+    ~list_step_start forms other_elm f 
+  `),
+  rw [] >>
+  Induct_on `forms`
+  >| [
+    rw [list_step_start_def]
+    ,
+
+    GEN_TAC >>
+    Cases_on `h = Not f`
+    >| [
+      `h <> f` by (fs [MEM_childforms_anti_refl_thm, mk_childforms_def]) >>
+      rw [list_step_start_def] >>
+      fs []
+      ,
+
+      DISCH_TAC >> POP_ASSUM (fn thm =>
+        ASSUME_TAC (REWRITE_RULE [list_wellformed_def] thm)
+      ) >>
+      fs [] >>
+
+      rw [Once list_step_start_def] >>
+      fs [] >>
+
+      `MEM (Not f) forms` by (metis_tac [list_step_start_constrained_thm]) >>
+      fs [EVERY_MEM] >>
+
+      qpat_assum `MEM (Not f) forms` (fn arg_thm =>
+      qpat_assum `∀f'. MEM f' forms ==> ~MEM h (mk_childforms f')` (fn thm =>
+        ASSUME_TAC (MP (Q.SPEC `Not f` thm) arg_thm)
+      )) >>
+      fs [mk_childforms_def] >>
+      fs [list_step_start_def] >>
+      rw [list_step_start_def] 
+    ]
+
+  ]
+)
+
+
+val list_step_start_Start_elim_thm = Q.store_thm (
+  "list_step_start_Start_elim_thm",
+  (`∀ forms f .
+    ~ list_step_start forms other_elm (Start f)
+  `),
+  rw [] >>
+  Induct_on `forms`
+  >| [
+    rw [list_step_start_def]
+    ,
+
+    GEN_TAC >>
+    Cases_on `h = Start f`
+    >| [
+      `h <> f` by (fs [MEM_childforms_anti_refl_thm, mk_childforms_def]) >>
+      rw [list_step_start_def] >>
+      fs []
+      ,
+
+      DISCH_TAC >> POP_ASSUM (fn thm =>
+        ASSUME_TAC (REWRITE_RULE [list_wellformed_def] thm)
+      ) >>
+      fs [] >>
+
+      fs [Once list_step_start_def] >>
+      metis_tac []
+    ]
+  ]
+)
+
+val list_step_start_End_elim_thm = Q.store_thm (
+  "list_step_start_End_elim_thm",
+  (`∀ forms f .
+    ~ list_step_start forms other_elm (End f)
+  `),
+  rw [] >>
+  Induct_on `forms`
+  >| [
+    rw [list_step_start_def]
+    ,
+
+    GEN_TAC >>
+    Cases_on `h = End f`
+    >| [
+      `h <> f` by (fs [MEM_childforms_anti_refl_thm, mk_childforms_def]) >>
+      rw [list_step_start_def] >>
+      fs []
+      ,
+
+      DISCH_TAC >> POP_ASSUM (fn thm =>
+        ASSUME_TAC (REWRITE_RULE [list_wellformed_def] thm)
+      ) >>
+      fs [] >>
+
+      fs [Once list_step_start_def] >>
+      metis_tac []
+    ]
+  ]
+)
+
+
+
+val list_step_start_MEM_transition_start_eq_thm = Q.store_thm (
+  "list_step_start_MEM_transition_start_eq_thm",
+  (`∀ form forms .
+    list_wellformed forms ==>
+    (
+      list_step_start forms other_elm form <=>
+      MEM form (transition_start_rec forms other_elm)
+    )
+  `),
+  Induct_on `forms`
+  >| [
+    fs [list_step_start_def] >>
+    fs [transition_start_rec_def] >>
+    fs [empty_state_def]
+    ,
+    
+    GEN_TAC >> GEN_TAC >>
+    (Cases_on `form <> h` >- rw [list_wellformed_def, list_step_start_def, transition_start_rec_def]) >>
+    fs [] >>
+    rw [list_wellformed_def] >>
+    fs [] >>
+    qpat_x_assum `∀ form . list_step_start _ _ _ <=> MEM _ _` (fn rw_thm =>
+       ASSUME_TAC (GSYM rw_thm)
+    ) >>
+    Cases_on `form`
+    >| [
+      rw [list_step_start_def, transition_start_rec_def, decide_formula_start_def] >>
+      rw [list_step_start_Eid_elim_thm]
+      ,
+
+      rw [list_step_start_def, transition_start_rec_def, decide_formula_start_def] >>
+      rw [list_step_start_Prim_false_elim_thm]
+      ,
+
+      rw [transition_start_rec_def, decide_formula_start_def, list_step_start_def] >>
+      metis_tac [list_step_start_Imp_elim_thm]
+      ,
+
+      rw [transition_start_rec_def, decide_formula_start_def, list_step_start_def] >>
+      metis_tac [list_step_start_Equiv_elim_thm]
+      ,
+
+      rw [transition_start_rec_def, decide_formula_start_def, list_step_start_def] >>
+      metis_tac [list_step_start_Or_elim_thm]
+      ,
+
+      rw [transition_start_rec_def, decide_formula_start_def, list_step_start_def] >>
+      metis_tac [list_step_start_Xor_elim_thm]
+      ,
+
+      rw [transition_start_rec_def, decide_formula_start_def, list_step_start_def] >>
+      metis_tac [list_step_start_And_elim_thm]
+      ,
+
+      rw [transition_start_rec_def, decide_formula_start_def, list_step_start_def] >>
+      metis_tac [list_step_start_Since_elim_thm]
+      ,
+
+      rw [transition_start_rec_def, decide_formula_start_def, list_step_start_def] >>
+      metis_tac [list_step_start_Histor_elim_thm]
+      ,
+
+      rw [transition_start_rec_def, decide_formula_start_def, list_step_start_def] >>
+      metis_tac [list_step_start_Once_elim_thm]
+      ,
+
+      rw [transition_start_rec_def, decide_formula_start_def, list_step_start_def] >>
+      metis_tac [list_step_start_Prev_elim_thm]
+      ,
+
+      rw [transition_start_rec_def, decide_formula_start_def, list_step_start_def] >>
+      metis_tac [list_step_start_Start_elim_thm]
+      ,
+
+      rw [transition_start_rec_def, decide_formula_start_def, list_step_start_def] >>
+      metis_tac [list_step_start_End_elim_thm]
+      ,
+
+      rw [transition_start_rec_def, decide_formula_start_def, list_step_start_def] >>
+      metis_tac [list_step_start_Not_elim_thm]
+    ]
+  ]
+)
+
+
+val list_step_start_APPEND_thm = Q.store_thm (
+  "list_step_start_APPEND_thm",
+  (`∀ fs form' fs' .
+    list_wellformed fs ==>
+    list_wellformed fs' ==>
+    MEM form' fs' ==>
+    (
+      list_step_start (FILTER (\ x . ~ MEM x fs') fs ++ fs') other_elm form' <=>
+      list_step_start fs' other_elm form'
+    )
+  `),
+  GEN_TAC >> GEN_TAC >> GEN_TAC >>
+  (Induct_on `fs` >- rw []) >>
+  GEN_TAC >>
+
+  rw [Once list_wellformed_def] >>
+  (Cases_on `h = form'` >- fs []) >>
+  rw [Once list_step_start_def]
+)
+
+
+val list_wellformed_childform_included_thm = Q.store_thm (
+  "list_wellformed_childform_included_thm",
+  (`∀ fs f f' .
+    list_wellformed fs ==>
+    MEM f fs ==>
+    MEM f' (mk_childforms f) ==>
+    MEM f' fs
+  `),
+  rw [] >>
+  (Induct_on `fs` >- rw []) >>
+  GEN_TAC >>
+  rw [Once list_wellformed_def, EVERY_MEM] >> fs []
+)
+
+
+
+val list_wellformed_append_thm = Q.store_thm (
+  "list_wellformed_append_thm",
+  (`∀ fs fs' .
+    list_wellformed fs ==>
+    list_wellformed fs' ==>
+    list_wellformed ((FILTER (\ x. ~MEM x fs') fs) ⧺ fs')
+  `),
+  rw [] >>
+  (Induct_on `fs` >- rw []) >>
+  GEN_TAC >>
+  rw [Once list_wellformed_def] >>
+  fs [EVERY_MEM] >>
+  rw [Once list_wellformed_def, EVERY_MEM]
+  >| [
+    qpat_x_assum `∀ f' . MEM f' (mk_childforms h) ==> _` (fn thm =>
+      ASSUME_TAC (Q.SPEC `f'` thm)
+    ) >>
+
+    qpat_assum `MEM f' (mk_childforms h)` (fn arg_thm =>
+    qpat_assum `MEM f' (mk_childforms h) ==> _` (fn imp_thm =>
+      ASSUME_TAC (MP imp_thm arg_thm)
+    )) >>
+
+    fs [MEM_FILTER]
+    ,
+
+    `MEM f' fs` by (fs [MEM_FILTER]) >>
+    qpat_x_assum `∀ f' . MEM f' fs ==> _` (fn thm =>
+      ASSUME_TAC (Q.SPEC `f'` thm)
+    ) >>
+
+    qpat_assum `MEM f' fs` (fn arg_thm =>
+    qpat_assum `MEM f' fs ==> _` (fn imp_thm =>
+      ASSUME_TAC (MP imp_thm arg_thm)
+    )) >>
+
+    fs []
+    ,
+
+    metis_tac [list_wellformed_childform_included_thm]
+    ,
+
+    fs [MEM_FILTER]
+  ]
+)
+
+val list_wellformed_nub_subforms_thm = Q.store_thm (
+  "list_wellformed_nub_subforms_thm",
+  `∀ form . list_wellformed (nub (mk_subforms form))`,
+  Induct_on `form`
+  >| [
+    rw [mk_subforms_def, nub_def, list_wellformed_def, mk_childforms_def]
+    ,
+
+    rw [mk_subforms_def, nub_def, list_wellformed_def, mk_childforms_def]
+    ,
+
+    `~ MEM (Imp form form') (mk_subforms form)` by (fs [MEM_subforms_acyclic_thm, mk_childforms_def]) >>
+    `~ MEM (Imp form form') (mk_subforms form')` by (fs [MEM_subforms_acyclic_thm, mk_childforms_def]) >>
+    rw [Once mk_subforms_def, nub_def] >>
+    rw [Once list_wellformed_def]
+    >| [
+      rw [mk_childforms_def] >> rw [MEM_subforms_self_thm]
+      ,
+      rw [EVERY_MEM] >> ( 
+        DISCH_TAC >>
+        `~MEM f' (mk_subforms (Imp form form'))` by (metis_tac [MEM_subforms_acyclic_thm]) >>
+        fs [Once mk_subforms_def]
+      )
+      ,
+
+      rw [nub_append, GSYM FILTER_nub_thm] >>
+      `(\ x. ~ MEM x (mk_subforms form')) = (\ x. ~ MEM x (nub (mk_subforms form')))` by (
+        fs [Once (GSYM MEM_nub_thm)]
+      ) >>
+      POP_ASSUM (fn rw_thm => FULL_SIMP_TAC std_ss [Once rw_thm]) >>
+      rw [list_wellformed_append_thm]
+    
+    ]
+    ,
+
+    `~ MEM (Equiv form form') (mk_subforms form)` by (fs [MEM_subforms_acyclic_thm, mk_childforms_def]) >>
+    `~ MEM (Equiv form form') (mk_subforms form')` by (fs [MEM_subforms_acyclic_thm, mk_childforms_def]) >>
+    rw [Once mk_subforms_def, nub_def] >>
+    rw [Once list_wellformed_def]
+    >| [
+      rw [mk_childforms_def] >> rw [MEM_subforms_self_thm]
+      ,
+      rw [EVERY_MEM] >> ( 
+        DISCH_TAC >>
+        `~MEM f' (mk_subforms (Equiv form form'))` by (metis_tac [MEM_subforms_acyclic_thm]) >>
+        fs [Once mk_subforms_def]
+      )
+      ,
+
+      rw [nub_append, GSYM FILTER_nub_thm] >>
+      `(\ x. ~ MEM x (mk_subforms form')) = (\ x. ~ MEM x (nub (mk_subforms form')))` by (
+        fs [Once (GSYM MEM_nub_thm)]
+      ) >>
+      POP_ASSUM (fn rw_thm => FULL_SIMP_TAC std_ss [Once rw_thm]) >>
+      rw [list_wellformed_append_thm]
+    
+    ]
+    ,
+
+    `~ MEM (Or form form') (mk_subforms form)` by (fs [MEM_subforms_acyclic_thm, mk_childforms_def]) >>
+    `~ MEM (Or form form') (mk_subforms form')` by (fs [MEM_subforms_acyclic_thm, mk_childforms_def]) >>
+    rw [Once mk_subforms_def, nub_def] >>
+    rw [Once list_wellformed_def]
+    >| [
+      rw [mk_childforms_def] >> rw [MEM_subforms_self_thm]
+      ,
+      rw [EVERY_MEM] >> ( 
+        DISCH_TAC >>
+        `~MEM f' (mk_subforms (Or form form'))` by (metis_tac [MEM_subforms_acyclic_thm]) >>
+        fs [Once mk_subforms_def]
+      )
+      ,
+
+      rw [nub_append, GSYM FILTER_nub_thm] >>
+      `(\ x. ~ MEM x (mk_subforms form')) = (\ x. ~ MEM x (nub (mk_subforms form')))` by (
+        fs [Once (GSYM MEM_nub_thm)]
+      ) >>
+      POP_ASSUM (fn rw_thm => FULL_SIMP_TAC std_ss [Once rw_thm]) >>
+      rw [list_wellformed_append_thm]
+    ]
+    ,
+
+    `~ MEM (Xor form form') (mk_subforms form)` by (fs [MEM_subforms_acyclic_thm, mk_childforms_def]) >>
+    `~ MEM (Xor form form') (mk_subforms form')` by (fs [MEM_subforms_acyclic_thm, mk_childforms_def]) >>
+    rw [Once mk_subforms_def, nub_def] >>
+    rw [Once list_wellformed_def]
+    >| [
+      rw [mk_childforms_def] >> rw [MEM_subforms_self_thm]
+      ,
+      rw [EVERY_MEM] >> ( 
+        DISCH_TAC >>
+        `~MEM f' (mk_subforms (Xor form form'))` by (metis_tac [MEM_subforms_acyclic_thm]) >>
+        fs [Once mk_subforms_def]
+      )
+      ,
+
+      rw [nub_append, GSYM FILTER_nub_thm] >>
+      `(\ x. ~ MEM x (mk_subforms form')) = (\ x. ~ MEM x (nub (mk_subforms form')))` by (
+        fs [Once (GSYM MEM_nub_thm)]
+      ) >>
+      POP_ASSUM (fn rw_thm => FULL_SIMP_TAC std_ss [Once rw_thm]) >>
+      rw [list_wellformed_append_thm]
+    ]
+    ,
+    
+    `~ MEM (And form form') (mk_subforms form)` by (fs [MEM_subforms_acyclic_thm, mk_childforms_def]) >>
+    `~ MEM (And form form') (mk_subforms form')` by (fs [MEM_subforms_acyclic_thm, mk_childforms_def]) >>
+    rw [Once mk_subforms_def, nub_def] >>
+    rw [Once list_wellformed_def]
+    >| [
+      rw [mk_childforms_def] >> rw [MEM_subforms_self_thm]
+      ,
+      rw [EVERY_MEM] >> ( 
+        DISCH_TAC >>
+        `~MEM f' (mk_subforms (And form form'))` by (metis_tac [MEM_subforms_acyclic_thm]) >>
+        fs [Once mk_subforms_def]
+      )
+      ,
+
+      rw [nub_append, GSYM FILTER_nub_thm] >>
+      `(\ x. ~ MEM x (mk_subforms form')) = (\ x. ~ MEM x (nub (mk_subforms form')))` by (
+        fs [Once (GSYM MEM_nub_thm)]
+      ) >>
+      POP_ASSUM (fn rw_thm => FULL_SIMP_TAC std_ss [Once rw_thm]) >>
+      rw [list_wellformed_append_thm]
+    ]
+    ,
+
+    `~ MEM (Since form form') (mk_subforms form)` by (fs [MEM_subforms_acyclic_thm, mk_childforms_def]) >>
+    `~ MEM (Since form form') (mk_subforms form')` by (fs [MEM_subforms_acyclic_thm, mk_childforms_def]) >>
+    rw [Once mk_subforms_def, nub_def] >>
+    rw [Once list_wellformed_def]
+    >| [
+      rw [mk_childforms_def] >> rw [MEM_subforms_self_thm]
+      ,
+      rw [EVERY_MEM] >> ( 
+        DISCH_TAC >>
+        `~MEM f' (mk_subforms (Since form form'))` by (metis_tac [MEM_subforms_acyclic_thm]) >>
+        fs [Once mk_subforms_def]
+      )
+      ,
+
+      rw [nub_append, GSYM FILTER_nub_thm] >>
+      `(\ x. ~ MEM x (mk_subforms form')) = (\ x. ~ MEM x (nub (mk_subforms form')))` by (
+        fs [Once (GSYM MEM_nub_thm)]
+      ) >>
+      POP_ASSUM (fn rw_thm => FULL_SIMP_TAC std_ss [Once rw_thm]) >>
+      rw [list_wellformed_append_thm]
+    ]
+    ,
+
+    `~ MEM (Histor form) (mk_subforms form)` by (fs [MEM_subforms_acyclic_thm, mk_childforms_def]) >>
+    rw [Once mk_subforms_def, nub_def] >>
+    rw [Once list_wellformed_def]
+    >| [
+      rw [mk_childforms_def] >> rw [MEM_subforms_self_thm]
+      ,
+      rw [EVERY_MEM] >> ( 
+        DISCH_TAC >>
+        `~MEM f' (mk_subforms (Histor form))` by (metis_tac [MEM_subforms_acyclic_thm]) >>
+        fs [Once mk_subforms_def]
+      )
+    ]
+    ,
+
+    `~ MEM (Once form) (mk_subforms form)` by (fs [MEM_subforms_acyclic_thm, mk_childforms_def]) >>
+    rw [Once mk_subforms_def, nub_def] >>
+    rw [Once list_wellformed_def]
+    >| [
+      rw [mk_childforms_def] >> rw [MEM_subforms_self_thm]
+      ,
+      rw [EVERY_MEM] >> ( 
+        DISCH_TAC >>
+        `~MEM f' (mk_subforms (Once form))` by (metis_tac [MEM_subforms_acyclic_thm]) >>
+        fs [Once mk_subforms_def]
+      )
+    ]
+    ,
+
+    `~ MEM (Prev form) (mk_subforms form)` by (fs [MEM_subforms_acyclic_thm, mk_childforms_def]) >>
+    rw [Once mk_subforms_def, nub_def] >>
+    rw [Once list_wellformed_def]
+    >| [
+      rw [mk_childforms_def] >> rw [MEM_subforms_self_thm]
+      ,
+      rw [EVERY_MEM] >> ( 
+        DISCH_TAC >>
+        `~MEM f' (mk_subforms (Prev form))` by (metis_tac [MEM_subforms_acyclic_thm]) >>
+        fs [Once mk_subforms_def]
+      )
+    ]
+    ,
+
+    `~ MEM (Start form) (mk_subforms form)` by (fs [MEM_subforms_acyclic_thm, mk_childforms_def]) >>
+    rw [Once mk_subforms_def, nub_def] >>
+    rw [Once list_wellformed_def]
+    >| [
+      rw [mk_childforms_def] >> rw [MEM_subforms_self_thm]
+      ,
+      rw [EVERY_MEM] >> ( 
+        DISCH_TAC >>
+        `~MEM f' (mk_subforms (Start form))` by (metis_tac [MEM_subforms_acyclic_thm]) >>
+        fs [Once mk_subforms_def]
+      )
+    ]
+    ,
+
+    `~ MEM (End form) (mk_subforms form)` by (fs [MEM_subforms_acyclic_thm, mk_childforms_def]) >>
+    rw [Once mk_subforms_def, nub_def] >>
+    rw [Once list_wellformed_def]
+    >| [
+      rw [mk_childforms_def] >> rw [MEM_subforms_self_thm]
+      ,
+      rw [EVERY_MEM] >> ( 
+        DISCH_TAC >>
+        `~MEM f' (mk_subforms (End form))` by (metis_tac [MEM_subforms_acyclic_thm]) >>
+        fs [Once mk_subforms_def]
+      )
+    ]
+    ,
+
+    `~ MEM (Not form) (mk_subforms form)` by (fs [MEM_subforms_acyclic_thm, mk_childforms_def]) >>
+    rw [Once mk_subforms_def, nub_def] >>
+    rw [Once list_wellformed_def]
+    >| [
+      rw [mk_childforms_def] >> rw [MEM_subforms_self_thm]
+      ,
+      rw [EVERY_MEM] >> ( 
+        DISCH_TAC >>
+        `~MEM f' (mk_subforms (Not form))` by (metis_tac [MEM_subforms_acyclic_thm]) >>
+        fs [Once mk_subforms_def]
+      )
+    ]
+  ]
+)
+
+
+(* SCRATCH: *)
+
+
+
+val list_wellformed_subforms_elim_thm = Q.store_thm (
+  "list_wellformed_subforms_thm",
+  (`∀ fs1 fs2 . 
+    list_wellformed fs ==>
+    MEM f fs ==>
+    EVERY (\ f' . MEM f' fs) (mk_subforms f)
+  `),
+  (* TODO *)
+  cheat
+)
+
+
+val list_step_start_FILTER_APPEND_thm = Q.store_thm (
+  "list_step_start_FILTER_APPEND_thm",
+  (`∀ form fs fs' .
+    list_wellformed fs ==>
+    list_wellformed fs' ==>
+    MEM form fs ==>
+    (
+      list_step_start (FILTER (\ x . ~ MEM x fs') fs ++ fs') other_elm form <=>
+      list_step_start fs other_elm form
+    )
+  `),
+  rw [] >>
+  (* TODO *)
+  cheat
+)
+
+
+
+
+val list_step_start_imp_gen_thm = Q.store_thm (
+  "list_step_start_imp_gen_thm",
+  (`∀ form fs form' fs' .
+    list_wellformed fs ==>
+    MEM form fs ==>
+    list_wellformed fs' ==>
+    MEM form' fs' ==>
+    (
+      (list_step_start
+        (Imp form form' :: (FILTER (\x. ~MEM x fs') fs) ++ fs')
+        other_elm
+        (Imp form form')
+      ) <=> (
+        (list_step_start fs other_elm) form ==>
+        (list_step_start fs' other_elm) form'
+      )
+    )
+  `),
+
+  GEN_TAC >> GEN_TAC >> GEN_TAC >> GEN_TAC >>
+  rw [Once list_step_start_def] >>
+  fs [] >>
+
+  ASSUME_TAC list_step_start_APPEND_thm >> 
+  ASSUME_TAC list_step_start_FILTER_APPEND_thm >> 
+  fs [] >>
+  metis_tac []
+)
+
+val list_step_start_imp_thm = Q.store_thm (
+  "list_step_start_imp_thm",
+  (`∀ form form' .
+    (list_step_start (nub (mk_subforms (Imp form form'))) other_elm (Imp form form')) <=>
+    (
+      list_step_start (nub (mk_subforms form)) other_elm form ==>
+      list_step_start (nub (mk_subforms form')) other_elm form'
+    )
+  `),
+  GEN_TAC >> GEN_TAC >>
+  rw [Once mk_subforms_def] >>
+  FULL_SIMP_TAC std_ss [Once nub_def] >>
+
+  `~MEM (Imp form form') (mk_subforms form)` by (fs [MEM_subforms_acyclic_thm, mk_childforms_def]) >>
+  `~MEM (Imp form form') (mk_subforms form')` by (fs [MEM_subforms_acyclic_thm, mk_childforms_def]) >>
+  fs [] >>
+  fs [Once nub_append] >>
+  fs [Once (GSYM FILTER_nub_thm)] >>
+
+  `(\ x. ~ MEM x (mk_subforms form')) = (\ x. ~ MEM x (nub (mk_subforms form')))` by (
+    fs [Once (GSYM MEM_nub_thm)]
+  ) >>
+  POP_ASSUM (fn rw_thm => FULL_SIMP_TAC std_ss [Once rw_thm]) >>
+
+
+  `list_wellformed (nub (mk_subforms form))` by (fs [list_wellformed_nub_subforms_thm]) >>
+  `list_wellformed (nub (mk_subforms form'))` by (fs [list_wellformed_nub_subforms_thm]) >>
+
+  `∃ fs . nub (mk_subforms form) = fs /\ MEM form fs` by (fs [nub_subforms_MEM_thm]) >>
+  `∃ fs' . nub (mk_subforms form') = fs' /\ MEM form' fs'` by (fs [nub_subforms_MEM_thm]) >>
+  FULL_SIMP_TAC std_ss [] >>
+  ASSUME_TAC (list_step_start_imp_gen_thm) >>
+  fs []
+)  
+
+
+  `form = form' ==> nub (mk_subforms form) = nub (mk_subforms form')` by (fs []) >>
+
+val bigstep_equiv_smallstep_empty_trace_thm = Q.store_thm (
+ "bigstep_equiv_smallstep_empty_trace_thm",
+ `∀ form . bigstep form [] <=> smallstep form []`,
+
+  GEN_TAC >>
+  fs [Once smallstep_def] >> fs [transition_start_REVERSE_rec_equiv_thm] >>
+  fs [GSYM (MP 
+   (Q.SPECL [`form`, `nub (mk_subforms form)`] list_step_start_MEM_transition_start_eq_thm)
+   (Q.SPEC `form `list_wellformed_nub_subforms_thm)
+  )] >>
+
+  Induct_on `form`
+  >| [
+    rw [
+      bigstep_def, other_elm_def, mk_subforms_def,
+      nub_def, list_step_start_def,
+      empty_state_def
+    ]
+    ,
+
+    rw [
+      bigstep_def, other_elm_def, mk_subforms_def,
+      nub_def, list_step_start_def,
+      empty_state_def
+    ]
+    ,
+
+    rw [Once bigstep_def] >>
+    metis_tac [list_step_start_imp_thm]
+    ,
+
+    (* TODO *)
+    cheat
+    ,
+
+    (* TODO *)
+    cheat
+    ,
+
+    (* TODO *)
+    cheat
+    ,
+
+    (* TODO *)
+    cheat
+    ,
+
+    (* TODO *)
+    cheat
+    ,
+
+    (* TODO *)
+    cheat
+    ,
+
+    (* TODO *)
+    cheat
+    ,
+
+    (* TODO *)
+    cheat
+    ,
+
+    (* TODO *)
+    cheat
+    ,
+
+    (* TODO *)
+    cheat
+    ,
+
+    (* TODO *)
+    cheat
+ ]
+ 
+)
+
+
+val bigstep_equiv_smallstep_thm = Q.store_thm (
+ "bigstep_equiv_smallstep_thm",
+ `∀ form trace . bigstep form trace <=> smallstep form trace`,
+ Cases_on `trace` >| [
+   (* TODO *)
+ ]
+)
+
+
+val smallstep_equiv_dfa_thm = Q.store_thm (
+ "smallstep_equiv_dfa_thm",
+ `∀ form trace . smallstep form trace <=> dfa form trace`,
+ (* TODO *)
+)
+
+
+
+val bigtep_equiv_dfa_thm = Q.store_thm (
+ "bigtep_equiv_dfa_thm",
+ `∀ form trace . bigstep form trace <=> dfa form trace`,
+ (* TODO *)
+)
+
+
 
 val _ = export_theory();
