README.md
@@ -16,19 +16,19 @@ Retdec - https://retdec.com/
 ### PTLTL 
 The specification `histor ((b --> prev (~b since a)) /\ ~(a /\ b))` is stored in `specs/ptltl/spec_1.pt`.  It says that if there is a `b` then the preceding tokens since an `a` are not `b`s, and their was certainly a preceding `a`.  Additionally, `a` and `b` cannot occur simultaneously.
 
-# build step
+#### build step
 ```bash
 $ cd code-hol4/ptltl
 $ Holmake
 ```
-# synthesis step
+#### synthesis step
 ```bash
 $ ./synthesize.sh tablestep_monitor ../../specs/ptltl/spec_1.pt
 ```
 multiple kinds of artifacts may be synthesized using the keywords `lex`, `gram`, `bigstep`, `smallstep`, `smallstep_monitor` and `tablestep_monitor`, and `dotgraph`.
 for each of `bigstep`, `smallstep`, `smallstep_monitor` and `tablestep_monitor`, 4 kinds of artifacts are produced with extensions `.cakeml.sexp`, `.S`, `.exe`, and `.C`.
 
-# run step
+#### run step
 ```bash
 $ ../../specs/ptltl/spec_1.pt.tablestep_monitor.exe
 > a a a
@@ -48,3 +48,96 @@ REJECTED
 Example specifications are in `specs/ptltl`.  The tokens are separated by white space.  A token containing words with dots in between means that each word of that token is active simultaneously.  That is, the formula accepts the token if the formula requires a subset of those words.  
 
 The smallstep DFA synthesis is based on Havelund/Rosu's ["Synthesizing Monitors for Safety Properties"](https://ti.arc.nasa.gov/m/pub-archive/345h/0345%20(Havelund).pdf)  
+
+
+#### PTLTL Proof Story
+
+The top level correctness theorems state the equivalence between three defintions of
+PTLTL machines: bigstep, smallstep, and dfa.
+```
+∀ form trace . bigstep form trace <=> smallstep form trace
+
+∀ form trace . smallstep form trace <=> dfa form trace
+
+∀ form trace . bigstep form trace <=> dfa form trace
+```
+
+smallstep is defined in terms of transition functions, each over a list of subformulas.
+The transition functions are transition_start and transition.  
+These are defined using FOLDL for speed.  For proof, it's useful to find an equivalent defintion that is structurally recursive over the list.
+
+```
+∀ sforms elm . transition_start (REVERSE sforms) elm = transition_start_rec sforms elm
+```
+
+The resulting value of the smallstep is the same as the membership of a formula in the result of the transition
+functions.  To make reasoning over this easier, a more direct recursive boolean function called is used.
+
+```
+∀ form forms .
+  list_wellformed forms ==> (
+    list_step_start forms other_elm form <=> MEM form (transition_start_rec forms other_elm)
+  )
+  
+```
+
+bigstep is structural recursive over formulas, which is structurally binary trees.
+formulas map to a corresponding operation in the host logic.
+e.g. for implication:
+```
+∀ f1 f2 . bigstep (Imp f1 f2) <=> (bigstep f1 trace ==> bigstep f2 trace)
+```
+
+To show equivalence between bigstep and smallstep, we show that smallstep definitions can maintain
+isomorphic mappings to the host logic.
+```
+∀ form form' .
+  (list_step_start (nub (mk_subforms (Imp form form'))) other_elm (Imp form form')) <=>
+  (
+    list_step_start (nub (mk_subforms form)) other_elm form ==>
+    list_step_start (nub (mk_subforms form')) other_elm form'
+  )
+```
+
+Since transition_start_rec is structurally recursive over lists, but formulas are binary trees,
+inducting over formulas won't work.  Instead we neew a way to characterize the list that's produced by
+`mk_subforms`. `list_wellformed` is an attempt at this.  It states that if a formula exists in a list, then its subformulas exist in the remainder of the list.  Additionaly, the formula cannot be a child or equal to any formula in the remainder of the list, which entails that it cannot be a subform of any formula, since all children, and children of children, etc, are required to be in the list.     
+Given list_wellformed is implied by mk_subforms, we can generalize:
+```
+∀ form fs form' fs' .
+  list_wellformed fs ==>
+  MEM form fs ==>
+  list_wellformed fs' ==>
+  MEM form' fs' ==>
+  (
+    (list_step_start
+      (Imp form form' :: (FILTER (\x. ~MEM x fs') fs) ++ fs')
+      other_elm
+      (Imp form form')
+    ) <=> (
+      (list_step_start fs other_elm) form ==>
+      (list_step_start fs' other_elm) form'
+    )
+  )
+```
+
+#### PTLTL Proof Dead Ends and Obstacles 
+A handful of stragies were too difficult or infeasable.
+
+ - Splitting equivalence into two implication lemmas. 
+   - This weakened the induction hypothesis too much.
+
+ - Inducting over FOLDL and characterizing the accumulator and the subforms list input.
+   - This was too cumbersome. Switching to a natural recursive defintion appears simpler and removes the need for reversing the list.
+
+ - Defining using case operater instead of parameter patterns  
+   - This complicated rewriting
+ 
+
+
+
+
+
+
+
+
